@prefix cco: <http://data.bioversityinternational.org/cco#>.
@prefix rdf: <http://www.w3.org/1999/02/22-rdf-syntax-ns#>.
@prefix rdfs: <http://www.w3.org/2000/01/rdf-schema#>.
@prefix foaf: <http://xmlns.com/foaf/0.1/> .
@prefix xsd: <http://www.w3.org/2001/XMLSchema#>.
@prefix owl:  <http://www.w3.org/2002/07/owl#> .
@prefix dc:      <http://purl.org/dc/elements/1.1/> .
@prefix book: <http://purl.org/NET/book/vocab#> .
   
cco:  a owl:Ontology ;
      dc:created "2013/09/23 12:00:00";
      dc:date "2013/09/23 12:00:00";
      dc:description """The Crop Characterization Ontology provides main concepts and properties for describing the characteristics of various crops. These concepts enable an easy and quick discrimination between phenotypes. They are generally highly heritable, can be easily seen by the eye and are equally expressed in all environments. In addition, these may include a limited number of additional traits thought desirable by a consensus of users of the particular crop.""" ;
      dc:title "The Crop Characterization Ontology" ;
      dc:hasVersion "Revision: 0.1" ;
      foaf:authors 
        [ foaf:name "Bioversity International"; foaf:homepage "http://www.bioversityinternational.org/" ];
      dc:contributor "Dr Silvio Belalcazar","Dr F. Carreel","Ching-Yan Tang","Dr Jeff Daniells","Prof. Bruno Delvaux","Mr Guy Evers","Dr Victor Galan Sauco","Dr Ricardo Goenaga","Prof. Oscar Haddad","Dr Yair Isralei","Mr Christophe Jenny","Mrs Deborah Karamura","Dr Emmanuel Lahav","Mr Christian Lavigne","Mr Thierry Lescot","Dr Rodomiro Ortiz","Mr Orlando C. Pascua","Mr Xavier Perrier","Dr Franklin Rosales","Ing. Irelio Sanchez Ramos","Prof Rony Swennen","Mr Hughes Tezenas du Montcel","Dr Kodjo Tomekpe", "Ir. Ines Van den houwe";
      dc:acknowledgments """IPGRI-INIBAP and CIRAD wish to place on record their sincere thanks to the numerous Musa workers around the world who have contributed directly or indirectly to the development of the Descriptors for banana. Mr H. Tezenas du Montcel, Mr C. Jenny and Dr X. Perrier from CIRAD-FLHOR have contributed to the development of the characterization form, which has been translated into English by Ms S. Sharrock (IBPGR) and into Spanish by Mr T. Lescot (CIRAD). Translation from French into English has been performed by Dr D.R. Jones, Ms E Arnaud and Dr J.P. Horry. Ms Adriana Alercia coordinated and supervised the text up to the pre-publication stage and provided technical advice. Ms Linda Sears edited the text and Ms Patrizia Tazza drew the cover, some illustrations, and prepared the layout. Scientific direction was provided by Dr Jean-Pierre Horry. Mr Paul Stapleton managed the production of the publication. Luca Matteis produced the underlying data model and the semantics of the ontology.""";
      foaf:page "http://data.bioversityinternational.org/cco";
      rdfs:seeAlso "http://www.bioversityinternational.org/e-library/publications/categories/descriptors/"
     .

cco:Characterization a rdfs:Class;
    rdfs:label "Characterization of crops"
    .

cco:Musa a rdfs:Class;
    rdfs:label "Musa spp.";
    rdfs:subClassOf cco:Characterization;
    foaf:page <http://www.bioversityinternational.org/e-library/publications/detail/descriptors-for-banana-emmusaem-spp/>;
    foaf:depiction <http://www.agrobiodiversity.org/files/MusaPDF.jpg>;
    book:isbn "978-92-9043-307-1"
    .
        
cco:leafHabitMusa a rdf:Property;
    rdfs:label "Leaf habit"@en;
    rdfs:comment """1 Erect
2 Intermediate
3 Drooping
4 Other (e.g. very drooping, specify in descriptor Notes, 6.8)"""@en;
    rdfs:domain cco:Musa;
    rdfs:range xsd:string;
    cco:section "6.1.1";
    foaf:depiction <http://www.agrobiodiversity.org/files/leafHabit.png>
    .
    
cco:dwarfismMusa a rdf:Property;
    rdfs:label "Dwarfism"@en;
    rdfs:comment """1 Normal: leaves not overlapped and leaf ratio inferior to 2.5
2 Dwarf type: leaves strongly overlapped and leaf ratio superior
to 2.5"""@en;
    rdfs:domain cco:Musa;
    rdfs:range xsd:string;
    cco:section "6.1.2"
    .
    
cco:pseudostemHeightMusa a rdf:Property;
    rdfs:label "Pseudostem height [m]"@en;
    rdfs:comment """Recorded from the base of pseudostem to emerging point of the peduncle
1 ≤2
2 2.1 to 2.9
3 ≥3"""@en;
    rdfs:domain cco:Musa;
    rdfs:range xsd:string;
    cco:section "6.2.1";
    foaf:depiction <http://www.agrobiodiversity.org/files/PseudostemSuckers.png>
    .
    
    
cco:pseudostemAspectMusa a rdf:Property;
    rdfs:label "Pseudostem aspect"@en;
    rdfs:comment """Determined by the circumference at 100 cm
1 Slender
2 Normal
3 Robust"""@en;
    rdfs:domain cco:Musa;
    rdfs:range xsd:string;
    cco:section "6.2.2"
    .
    
    
cco:pseudostemColourMusa a rdf:Property;
    rdfs:label "Pseudostem colour"@en;
    rdfs:comment """Recorded without removing the external sheaths. The colour of oldest dry sheaths should not be considered.
1 Green-yellow
2 Medium green
3 Green
4 Dark green
5 Green-red
6 Red
7 Red-purple
8 Blue
9 Chimerical
10 Other"""@en;
    rdfs:domain cco:Musa;
    rdfs:range xsd:string;
    cco:section "6.2.3"
    .
    
    
cco:pseudostemAppearanceMusa a rdf:Property;
    rdfs:label "Pseudostem appearance"@en;
    rdfs:comment """Recorded as in cco:pseudostemColourMusa
1 Dull (waxy)
2 Shiny (not waxy)"""@en;
    rdfs:domain cco:Musa;
    rdfs:range xsd:string;
    cco:section "6.2.4"
    .
    
    
cco:predominantUnderlyingColourPseudostemMusa a rdf:Property;
    rdfs:label "Predominant underlying colour of the pseudostem"@en;
    rdfs:comment """Remove the outermost sheath from the pseudostem and look at the exposed surface
of the underlying pseudostem. The values 5 (pink-purple), 6 (red-purple) and 7
(purple) must be chosen only if the pigmentation is uniform, and green tinges are
not observed.
1 Watery green
2 Light green
3 Green
4 Cream
5 Pink-purple
6 Red-purple
7 Purple
8 Other"""@en;
    rdfs:domain cco:Musa;
    rdfs:range xsd:string;
    cco:section "6.2.5"
    .
    
cco:pigmentationUnderlyingPseudostemMusa a rdf:Property;
    rdfs:label "Pigmentation of the underlying pseudostem"@en;
    rdfs:comment """Record the tinge of pigmentation, even if it is only noticeable in places.
1 Pink-purple
2 Red
3 Purple
4 Other"""@en;
    rdfs:domain cco:Musa;
    rdfs:range xsd:string;
    cco:section "6.2.6"
    .
    
    

cco:sapColourMusa a rdf:Property;
    rdfs:label "Sap colour"@en;
    rdfs:comment """Cut the external sheath of pseudostem and record the characteristics of the sap.
1 Watery
2 Milky
3 Red-purple
4 Other"""@en;
    rdfs:domain cco:Musa;
    rdfs:range xsd:string;
    cco:section "6.2.7"
    .
    
    
cco:waxLeafSheathsMusa a rdf:Property;
    rdfs:label "Wax on leaf sheaths"@en;
    rdfs:comment """1 Very little or no visible sign of wax
2 Very few wax
3 Moderately waxy
4 Very waxy"""@en;
    rdfs:domain cco:Musa;
    rdfs:range xsd:string;
    cco:section "6.2.8"
    .
    
    
cco:numberOfSuckersMusa a rdf:Property;
    rdfs:label "Number of suckers"@en;
    rdfs:comment """Record the number of suckers from soil level to point of emergence of the last leaf
(>30 cm height). Recorded only if no desuckering has taken place"""@en;
    rdfs:domain cco:Musa;
    rdfs:range xsd:string;
    cco:section "6.2.9"
    .
    
cco:developmentOfSuckersMusa a rdf:Property;
    rdfs:label "Development of suckers"@en;
    rdfs:comment """In relation to the parent plant. Observed on the tallest sucker. Recorded at harvest
time
1 Taller than parent plant
2 More than 3/4 of the height of the parent plant
3 Between 1/4 and 3/4 of the height of the parent plant
4 Inhibited"""@en;
    rdfs:domain cco:Musa;
    rdfs:range xsd:string;
    cco:section "6.2.10"
    .

cco:positionOfSuckersMusa a rdf:Property;
    rdfs:label "Position of suckers"@en;
    rdfs:comment """1 Far from parent plant (emerging >50 cm from parent plant)
2 Close to parent (vertical growth)
3 Close to parent (growing at an angle)"""@en;
    rdfs:domain cco:Musa;
    rdfs:range xsd:string;
    cco:section "6.2.11"
    .
cco:blotchesPetioleBaseMusa a rdf:Property;
    rdfs:label "Blotches at the petiole base"@en;
    rdfs:comment """Recorded on the third, fully unfolded leaf counting down from the top of the plant.
    
1 Sparse blotching
2 Small blotches
3 Large blotches
4 Extensive pigmentation
5 Without pigmentation"""@en;
    rdfs:domain cco:Musa;
    rdfs:range xsd:string;
    cco:section "6.3.1";
    foaf:depiction <http://www.agrobiodiversity.org/files/PetioleMidribLeaf.png>
    .
    
    
cco:blotchesColourMusa a rdf:Property;
    rdfs:label "Blotches colour"@en;
    rdfs:comment """1 Brown
2 Dark brown
3 Brown-black
4 Black-purple
5 Other"""@en;
    rdfs:domain cco:Musa;
    rdfs:range xsd:string;
    cco:section "6.3.2"
    .
    
cco:petioleCanalLeafIIIMusa a rdf:Property;
    rdfs:label "Petiole canal leaf III"@en;
    rdfs:comment """Leaf III is the third leaf counted from the last leaf (leaf I) produced before bunch
emergence. Cut the petiole half way between the pseudostem and the leaf blade
and examine the cross section.

1 Open with margins spreading
2 Wide with erect margins
3 Straight with erect margins
4 Margins curved inward
5 Margins overlapping"""@en;
    rdfs:domain cco:Musa;
    rdfs:range xsd:string;
    cco:section "6.3.3";
    foaf:depiction <http://www.agrobiodiversity.org/files/petioleCanalLeafIIIMusa.png>
    .


cco:petioleMarginsMusa a rdf:Property;
    rdfs:label "Petiole margins"@en;
    rdfs:comment """1 Winged and undulating
2 Winged and not clasping the pseudostem
3 Winged and clasping the pseudostem
4 Not winged and clasping the pseudostem
5 Not winged and not clasping the pseudostem"""@en;
    rdfs:domain cco:Musa;
    rdfs:range xsd:string;
    cco:section "6.3.4"
    .

cco:wingTypeMusa a rdf:Property;
    rdfs:label "Wing type"@en;
    rdfs:comment """
1 Dry
2 Not dry
    """@en;
    rdfs:domain cco:Musa;
    rdfs:range xsd:string;
    cco:section "6.3.5"
    .

cco:petioleMarginColourMusa a rdf:Property;
    rdfs:label "Petiole margin colour"@en;
    rdfs:comment """
1 Green
2 Pink-purple to red
3 Purple to blue
4 Other
    """@en;
    rdfs:domain cco:Musa;
    rdfs:range xsd:string;
    cco:section "6.3.6"
    .

cco:edgeOfPetioleMarginMusa a rdf:Property;
    rdfs:label "Edge of petiole margin"@en;
    rdfs:comment """
1 Colourless (without a colour line along)
2 With a colour line along
    """@en;
    rdfs:domain cco:Musa;
    rdfs:range xsd:string;
    cco:section "6.3.7"
    .

cco:petioleWarginWidthMusa a rdf:Property;
    rdfs:label "Petiole margin width"@en;
    rdfs:comment """
1 ≤1 cm
2 >1 cm
3 Cannot be defined
    """@en;
    rdfs:domain cco:Musa;
    rdfs:range xsd:string;
    cco:section "6.3.8"
    .


cco:leafBladeLengthMusa a rdf:Property;
    rdfs:label "Leaf blade length"@en;
    rdfs:comment """
Measured at its maximum point
1 ≤170 cm
2 171 to 220 cm
3 221 to 260 cm
4 ≥261 cm
    """@en;
    rdfs:domain cco:Musa;
    rdfs:range xsd:string;
    cco:section "6.3.9"
    .


cco:leafBladeWidthMusa a rdf:Property;
    rdfs:label "Leaf blade width"@en;
    rdfs:comment """
Measured at its maximum point
1 ≤70 cm
2 71 to 80 cm
3 81 to 90 cm
4 ≥91 cm
    """@en;
    rdfs:domain cco:Musa;
    rdfs:range xsd:string;
    cco:section "6.3.10"
    .

cco:leafRatioMusa a rdf:Property;
    rdfs:label "Leaf ratio"@en;
    rdfs:comment """
3 ≤2
5 2.4 to 2.6
7 ≥3
    """@en;
    rdfs:domain cco:Musa;
    rdfs:range xsd:string;
    cco:section "6.3.10.1"
    .

cco:petioleLengthMusa a rdf:Property;
    rdfs:label "Petiole length"@en;
    rdfs:comment """
Recorded from the pseudostem to the lamina
1 ≤50 cm
2 51 to 70 cm
3 ≥71 cm
    """@en;
    rdfs:domain cco:Musa;
    rdfs:range xsd:string;
    cco:section "6.3.11"
    .

cco:colourOfLeafUpperSurfaceMusa a rdf:Property;
    rdfs:label "Colour of leaf upper surface"@en;
    rdfs:comment """
1 Green-yellow
2 Medium green
3 Green
4 Dark green
5 Dark green with red-purple (presence of large blotches of
red-purple)
6 Blue
7 Other
    """@en;
    rdfs:domain cco:Musa;
    rdfs:range xsd:string;
    cco:section "6.3.12"
    .

cco:appearanceOfLeafUpperSurfaceMusa a rdf:Property;
    rdfs:label "Appearance of leaf upper surface"@en;
    rdfs:comment """
1 Dull
2 Shiny
    """@en;
    rdfs:domain cco:Musa;
    rdfs:range xsd:string;
    cco:section "6.3.13"
    .

cco:colourOfLeafLowerSurfaceMusa a rdf:Property;
    rdfs:label "Colour of leaf lower surface"@en;
    rdfs:comment """
1 Green-yellow 
2 Medium green 
3 Green
4 Dark green
5 Blue
6 Red-purple
7 Other
    """@en;
    rdfs:domain cco:Musa;
    rdfs:range xsd:string;
    cco:section "6.3.14"
    .

cco:appearanceOfLeafLowerSurfaceMusa a rdf:Property;
    rdfs:label "Appearance of leaf lower surface"@en;
    rdfs:comment """
1 Dull
2 Shiny
    """@en;
    rdfs:domain cco:Musa;
    rdfs:range xsd:string;
    cco:section "6.3.15"
    .


cco:waxOnLeavesMusa a rdf:Property;
    rdfs:label "Wax on leaves"@en;
    rdfs:comment """
Recorded on the lower surface
1 Very little or no visible sign of wax
2 Few wax
3 Moderately waxy
4 Very waxy
    """@en;
    rdfs:domain cco:Musa;
    rdfs:range xsd:string;
    cco:section "6.3.16"
    .

cco:insertionPointOfLeafBladesOnPetioleMusa a rdf:Property;
    rdfs:label "Insertion point of leaf blades on petiole"@en;
    rdfs:comment """
1 Symmetric
2 Asymmetric
    """@en;
    rdfs:domain cco:Musa;
    rdfs:range xsd:string;
    cco:section "6.3.17"
    .


cco:shapeOfLeafBladeBaseMusa a rdf:Property;
    rdfs:label "Shape of leaf blade base"@en;
    rdfs:comment """
1 Both sides rounded
2 One side rounded, one pointed
3 Both sides pointed
    """@en;
    rdfs:domain cco:Musa;
    rdfs:range xsd:string;
    cco:section "6.3.18";
    foaf:depiction <http://www.agrobiodiversity.org/files/shapeOfLeafBladeBase.png>
    .

cco:leafCorrugationMusa a rdf:Property;
    rdfs:label "Leaf corrugation"@en;
    rdfs:comment """
Presence of ridges perpendicular to the secondary ribs on the leaf upper surface
1 Even, smooth
2 Few stripes
3 Very corrugated
    """@en;
    rdfs:domain cco:Musa;
    rdfs:range xsd:string;
    cco:section "6.3.19"
    .

cco:colourOfMidribDorsalSurfaceMusa a rdf:Property;
    rdfs:label "Colour of midrib dorsal surface"@en;
    rdfs:comment """
If pigmentation is seen, options are 4, 5 or 6.
1 Yellow
2 Light green
3 Green
4 Pink-purple
5 Red-purple
6 Purple to blue
7 Other
    """@en;
    rdfs:domain cco:Musa;
    rdfs:range xsd:string;
    cco:section "6.3.20"
    .

cco:colourOfMidribVentralSurfaceMusa a rdf:Property;
    rdfs:label "Colour of midrib ventral surface"@en;
    rdfs:comment """
If pigmentation is seen, options are 4, 5 or 6.
1 Yellow
2 Light green
3 Green
4 Pink-purple
5 Red-purple
6 Purple to blue
7 Other
    """@en;
    rdfs:domain cco:Musa;
    rdfs:range xsd:string;
    cco:section "6.3.21"
    .

cco:colourOfCigarLeafDorsalSurfaceMusa a rdf:Property;
    rdfs:label "Colour of cigar leaf dorsal surface"@en;
    rdfs:comment """
Look at the visible face (future lower face) of the cigar leaf before it is unfurled and
before the plant flowers. (Chart A)
1 Green
2 Red-purple
3 Other (specify in descriptor Notes, 6.8)
    """@en;
    rdfs:domain cco:Musa;
    rdfs:range xsd:string;
    cco:section "6.3.22"
    .

cco:blotchesOnLeavesOfWaterSuckersMusa a rdf:Property;
    rdfs:label "Blotches on leaves of water suckers"@en;
    rdfs:comment """
Observed on young, non inhibited water suckers (if the lamina is sword shaped, it
is not a water sucker)
1 Without blotches
2 Little or narrow blotches
3 Large purple blotches
    """@en;
    rdfs:domain cco:Musa;
    rdfs:range xsd:string;
    cco:section "6.3.23"
    .



cco:peduncleLengthMusa a rdf:Property;
    rdfs:label "Peduncle length"@en;
    rdfs:comment """
Measured from the leaf crown to the first hand of fruit
1 ≤30 cm
2 31 - 60 cm
3 ≥61 cm
    """@en;
    rdfs:domain cco:Musa;
    rdfs:range xsd:string;
    cco:section "6.4.1"
    .

cco:emptyNodesOnPeduncleMusa a rdf:Property;
    rdfs:label "Empty nodes on peduncle"@en;
    rdfs:comment """
Record the number of empty nodes between the last bract-leaf and first hand of
fruit
    """@en;
    rdfs:domain cco:Musa;
    rdfs:range xsd:string;
    cco:section "6.4.2"
    .
    
cco:peduncleWidthMusa a rdf:Property;
    rdfs:label "Peduncle width"@en;
    rdfs:comment """
Recorded at mid-length
1 ≤6 cm
2 7 - 12 cm
3 ≥13 cm
    """@en;
    rdfs:domain cco:Musa;
    rdfs:range xsd:string;
    cco:section "6.4.3"
    .

cco:peduncleColourMusa a rdf:Property;
    rdfs:label "Peduncle colour"@en;
    rdfs:comment """
Descriptor state 4 (red/or pink-purple) is green homogeneously tinged with red
(purple green appearance). When pigmentation is scattered, use state 5. (Chart A)
1 Light green
2 Green
3 Dark green
4 Red or pink/purple
5 With purple-brown to blue blotches
6 Other
    """@en;
    rdfs:domain cco:Musa;
    rdfs:range xsd:string;
    cco:section "6.4.4"
    .

cco:peduncleHairinessMusa a rdf:Property;
    rdfs:label "Peduncle hairiness"@en;
    rdfs:comment """
1 Hairless
2 Slightly hairy
3 Very hairy, short hairs (similar to velvet touch)
4 Very hairy, long hairs (>2 mm)
    """@en;
    rdfs:domain cco:Musa;
    rdfs:range xsd:string;
    cco:section "6.4.5"
    .

cco:bunchPositionMusa a rdf:Property;
    rdfs:label "Bunch position"@en;
    rdfs:comment """
(Position of the fruit-bearing part). Angle from vertical to the general axis of the
bunch
1 Hanging vertically
2 Slightly angled
3 Hanging at angle 45°
4 Horizontal
5 Erect
    """@en;
    rdfs:domain cco:Musa;
    rdfs:range xsd:string;
    cco:section "6.4.6"
    .


cco:bunchShapeMusa a rdf:Property;
    rdfs:label "Bunch shape"@en;
    rdfs:comment """
1 Cylindrical
2 Truncated cone shape
3 Asymmetric - Bunch axis is nearly straight
4 With a curve in the bunch axis
5 Spiral (all fruit is attached to a unique crown coiled around the
stalk)
"""@en;
    rdfs:domain cco:Musa;
    rdfs:range xsd:string;
    cco:section "6.4.7"
    .

cco:bunchAppearanceMusa a rdf:Property;
    rdfs:label "Bunch appearance"@en;
    rdfs:comment """
1 Lax (one can easily place one’s hand between the
hands of fruit)
2 Compact (one can place one’s finger, but not one’s hand,
between the hands of fruit)
3 Very compact (one cannot place one’s finger between the hands
of fruit)
"""@en;
    rdfs:domain cco:Musa;
    rdfs:range xsd:string;
    cco:section "6.4.8"
    .

cco:flowersThatFormTheFruitMusa a rdf:Property;
    rdfs:label "Flowers that form the fruit"@en;
    rdfs:comment """
(4.2.3)
Record at flowering if the flowers of the first hands bear apparently functional
stamens
1 Female (absence of pollen sacs or pollens)
2 Hermaphrodite (presence of pollen sacs and pollens)
"""@en;
    rdfs:domain cco:Musa;
    rdfs:range xsd:string;
    cco:section "6.4.9"
    .

cco:fruitsMusa a rdf:Property;
    rdfs:label "Fruits"@en;
    rdfs:comment """
Positioning of fruits on the crown
1 Uniseriate
2 Biseriate
3 Biseriate and fused
"""@en;
    rdfs:domain cco:Musa;
    rdfs:range xsd:string;
    cco:section "6.4.10"
    .

cco:rachisTypeMusa a rdf:Property;
    rdfs:label "Rachis type"@en;
    rdfs:comment """
1 Truncated, no bract scar below the last hand of fruit
2 Present and male bud may be degenerated or persistent
"""@en;
    rdfs:domain cco:Musa;
    rdfs:range xsd:string;
    cco:section "6.4.11"
    .

cco:rachisPositionMusa a rdf:Property;
    rdfs:label "Rachis position"@en;
    rdfs:comment """
1 Falling vertically
2 At an angle
3 With a curve
4 Horizontal
5 Erect
"""@en;
    rdfs:domain cco:Musa;
    rdfs:range xsd:string;
    foaf:depiction <http://www.agrobiodiversity.org/files/rachisPosition.png>;
    cco:section "6.4.12"
    .

cco:rachisAppearanceMusa a rdf:Property;
    rdfs:label "Rachis appearance"@en;
    rdfs:comment """
1 Bare
2 Neutral flowers (one to few hands only, stalk is bare below)
3 Male flowers/bracts above the male bud (but the stalk is bare above
flowers/bracts)
4 Neutral/male flowers and presence of withered bracts (on the
whole stalk)
5 Neutral/male flowers on the whole stalk without persistent bracts
(e.g. AA var. ‘Tuu Gia’)
6 Small bunch from neutral/hermaphrodite flowers just above the
male bud (e.g. ABB var. ‘Monthan’)
7 Other (specify in descriptor 6.8, Notes)
    """@en;
    rdfs:domain cco:Musa;
    rdfs:range xsd:string;
    cco:section "6.4.13"
    .

cco:maleBudTypeMusa a rdf:Property;
    rdfs:label "Male bud type"@en;
    rdfs:comment """
Recorded at maturity
1 Normal (present)
2 Degenerating before maturity (like false-horn ‘Plantain’)
3 Like true-horn ‘Plantain’ (absent)
    """@en;
    rdfs:domain cco:Musa;
    rdfs:range xsd:string;
    cco:section "6.4.14"
    .

cco:maleBudShapeMusa a rdf:Property;
    rdfs:label "Male bud shape"@en;
    rdfs:comment """
Note the general shape of the male bud at harvest.
1 Like a top 
2 Lanceolate
3 Intermediate
4 Ovoid
5 Rounded
    """@en;
    rdfs:domain cco:Musa;
    rdfs:range xsd:string;
    foaf:depiction <http://www.agrobiodiversity.org/files/maleBudShape.png>;
    cco:section "6.4.15"
    .

cco:maleBudSizeMusa a rdf:Property;
    rdfs:label "Male bud size"@en;
    rdfs:comment """
Length and maximum diameter of male bud at harvest
1 ≤20 cm
2 21 to 30 cm
3 ≥31 cm
    """@en;
    rdfs:domain cco:Musa;
    rdfs:range xsd:string;
    cco:section "6.4.16"
    .


cco:bractBaseShapeMusa a rdf:Property;
    rdfs:label "Bract base shape"@en;
    rdfs:comment """
1 Small shoulder
2 Medium
3 Large shoulder
    """@en;
    rdfs:domain cco:Musa;
    rdfs:range xsd:string;
    foaf:depiction <http://www.agrobiodiversity.org/files/bractBaseShapeMusa.png>;
    cco:section "6.5.1"
    .

cco:bractApexShapeMusa a rdf:Property;
    rdfs:label "Bract apex shape"@en;
    rdfs:comment """
Flatten the apex of the bract to observe its shape.
1 Pointed
2 Slightly pointed
3 Intermediate
4 Obtuse
5 Obtuse and split
    """@en;
    rdfs:domain cco:Musa;
    rdfs:range xsd:string;
    foaf:depiction <http://www.agrobiodiversity.org/files/bractApexShapeMusa.png>;
    cco:section "6.5.2"
    .

cco:bractImbricationMusa a rdf:Property;
    rdfs:label "Bract imbrication"@en;
    rdfs:comment """
Note alignment of bracts at the apex of the male bud
1 Old bracts overlap at apex of bud (like Musa acuminata subsp. malaccensis)
2 Young bracts slightly overlap
3 Young bracts greatly overlap (like Musa acuminata subsp. burmanicca)
    """@en;
    rdfs:domain cco:Musa;
    rdfs:range xsd:string;
    cco:section "6.5.3"
    .


cco:colourOfTheBractExternalFaceMusa a rdf:Property;
    rdfs:label "Colour of the bract external face"@en;
    rdfs:comment """
1 Yellow 
2 Green 
3 Red 
4 Red-purple
5 Purple-brown
6 Purple
7 Blue
8 Pink-purple
9 Orange-red
10 Other
    """@en;
    rdfs:domain cco:Musa;
    rdfs:range xsd:string;
    cco:section "6.5.4"
    .

cco:colourOfTheBractInternalFaceMusa a rdf:Property;
    rdfs:label "Colour of the bract internal face"@en;
    rdfs:comment """
1 Whitish
2 Yellow or green 
3 Orange red 
4 Red 
5 Purple
6 Purple brown
7 Pink-purple
8 Other
    """@en;
    rdfs:domain cco:Musa;
    rdfs:range xsd:string;
    cco:section "6.5.5"
    .

cco:colourOnTheBractApexMusa a rdf:Property;
    rdfs:label "Colour on the bract apex"@en;
    rdfs:comment """
Recorded on the external face of the bract
1 Tinted with yellow (discoloured)
2 Not tinted with yellow (colour is uniform until apex)
    """@en;
    rdfs:domain cco:Musa;
    rdfs:range xsd:string;
    cco:section "6.5.6"
    .

cco:colourStripesOnBractMusa a rdf:Property;
    rdfs:label "Colour stripes on bract"@en;
    rdfs:comment """
1 Without discoloured lines (not ridges) on the external face
2 With discoloured lines or stripes on the external face
    """@en;
    rdfs:domain cco:Musa;
    rdfs:range xsd:string;
    cco:section "6.5.7"
    .

cco:bractScarsOnRachisMusa a rdf:Property;
    rdfs:label "Bract scars on rachis"@en;
    rdfs:comment """
Recorded on scars left after fall of bracts and flowers
1 Very prominent
2 Not prominent
    """@en;
    rdfs:domain cco:Musa;
    rdfs:range xsd:string;
    cco:section "6.5.8"
    .

cco:fadingOfColourOnBractBaseMusa a rdf:Property;
    rdfs:label "Fading of colour on bract base"@en;
    rdfs:comment """
Observed on the inside of the bract
1 Colour discontinuing towards the base (loss of pigmentation at the base)
2 Colour homogenous (pigmentation is uniform and continues until the base)
    """@en;
    rdfs:domain cco:Musa;
    rdfs:range xsd:string;
    cco:section "6.5.9"
    .

cco:maleBractShapeMusa a rdf:Property;
    rdfs:label "Male bract shape"@en;
    rdfs:comment """
1 x/y < 0.28 (Lanceolate)
2 0.28 < x/y <0.30
3 x/y > 0.30 (Ovate)
    """@en;
    rdfs:domain cco:Musa;
    rdfs:range xsd:string;
    foaf:depiction <http://www.agrobiodiversity.org/files/maleBractShapeMusa.png>;
    cco:section "6.5.10"
    .

cco:maleBractLiftingMusa a rdf:Property;
    rdfs:label "Male bract lifting"@en;
    rdfs:comment """
Number of raised bracts present on the male bud
1 Not lifting from male bud (bracts are persistent)
2 Lifting one at a time
3 Lifting two or more at a time
    """@en;
    rdfs:domain cco:Musa;
    rdfs:range xsd:string;
    cco:section "6.5.11"
    .

cco:bractBehaviourBeforeFallingMusa a rdf:Property;
    rdfs:label "Bract behaviour before falling"@en;
    rdfs:comment """
1 Revolute (rolling)
2 Not revolute (not rolling)
Fig. 13 Bract behaviour before falling
    """@en;
    rdfs:domain cco:Musa;
    rdfs:range xsd:string;
    foaf:depiction <http://www.agrobiodiversity.org/files/bractBehaviourBeforeFallingMusa.png>;
    cco:section "6.5.12"
    .

cco:waxOnTheBractMusa a rdf:Property;
    rdfs:label "Wax on the bract"@en;
    rdfs:comment """
Recorded on the external surface
1 Very little or no visible sign of wax
2 Very few wax
3 Moderately waxy
4 Very waxy
    """@en;
    rdfs:domain cco:Musa;
    rdfs:range xsd:string;
    cco:section "6.5.13"
    .

cco:presenceOfGroovesOnTheBractMusa a rdf:Property;
    rdfs:label "Presence of grooves on the bract"@en;
    rdfs:comment """
Observed on the external surface
1 Few grooves or not grooved (the bract is completely, or almost completely, smooth)
2 Moderate grooving (parallel ridges are distinguishable)
3 Strongly grooved (deep parallel furrows on the surface of bract)
    """@en;
    rdfs:domain cco:Musa;
    rdfs:range xsd:string;
    cco:section "6.5.14"
    .


cco:maleFlowerBehaviourMusa a rdf:Property;
    rdfs:label "Male flower behaviour"@en;
    rdfs:comment """
1 Falling before the bract
2 Falling with the bract
3 Falling after the bract
4 Neutral/male flowers persistent
    """@en;
    rdfs:domain cco:Musa;
    rdfs:range xsd:string;
    foaf:depiction <http://www.agrobiodiversity.org/files/maleFlowerMusa.png>;
    cco:section "6.6.1"
    .

cco:compoundTepalBasicColourMusa a rdf:Property;
    rdfs:label "Compound tepal basic colour"@en;
    rdfs:comment """
Without considering lobe colour.
1 White
2 Cream
3 Yellow
4 Orange
5 Pink/pink-purple
6 Other
    """@en;
    rdfs:domain cco:Musa;
    rdfs:range xsd:string;
    cco:section "6.6.2"
    .

cco:compoundTepalPigmentationMusa a rdf:Property;
    rdfs:label "Compound tepal pigmentation"@en;
    rdfs:comment """
1 Very few or no visible sign of pigmentation
2 Rust-coloured spots
3 Presence of pink
    """@en;
    rdfs:domain cco:Musa;
    rdfs:range xsd:string;
    cco:section "6.6.3"
    .

cco:lobeColourOfCompoundTepalMusa a rdf:Property;
    rdfs:label "Lobe colour of compound tepal"@en;
    rdfs:comment """
1 Cream
2 Yellow
3 Orange
4 Green
5 Other
    """@en;
    rdfs:domain cco:Musa;
    rdfs:range xsd:string;
    cco:section "6.6.4"
    .

cco:lobeDevelopmentOfCompoundTepalMusa a rdf:Property;
    rdfs:label "Lobe development of compound tepal"@en;
    rdfs:comment """
1 Little or not visible sign of development
2 Developed
3 Very developed
    """@en;
    rdfs:domain cco:Musa;
    rdfs:range xsd:string;
    cco:section "6.6.5"
    .

cco:freeTepalColourMusa a rdf:Property;
    rdfs:label "Free tepal colour"@en;
    rdfs:comment """
1 Translucent white
2 Opaque white
3 Tinted with yellow
4 Tinted with pink
    """@en;
    rdfs:domain cco:Musa;
    rdfs:range xsd:string;
    cco:section "6.6.6"
    .

cco:freeTepalShapeMusa a rdf:Property;
    rdfs:label "Free tepal shape"@en;
    rdfs:comment """
1 Rectangular
2 Oval
3 Rounded
4 Fan-shaped
    """@en;
    rdfs:domain cco:Musa;
    rdfs:range xsd:string;
    cco:section "6.6.7"
    .

cco:freeTepalAppearanceMusa a rdf:Property;
    rdfs:label "Free tepal appearance"@en;
    rdfs:comment """
1 Simple folding under apex
2 More or less smooth
3 Several folding under apex (corrugated)
    """@en;
    rdfs:domain cco:Musa;
    rdfs:range xsd:string;
    cco:section "6.6.8"
    .

 
cco:freeTepalApexDevelopmentMusa a rdf:Property;
    rdfs:label "Free tepal apex development"@en;
    rdfs:comment """
1 Little or no visible sign of development
2 Developed
3 Very developed
    """@en;
    rdfs:domain cco:Musa;
    rdfs:range xsd:string;
    foaf:depiction <http://www.agrobiodiversity.org/files/freeTepalApexDevelopmentMusa.png>;
    cco:section "6.6.9"
    .

cco:freeTepalApexShapeMusa a rdf:Property;
    rdfs:label "Free tepal apex shape"@en;
    rdfs:comment """
1 Thread-like
2 Triangular
3 Obtuse
    """@en;
    rdfs:domain cco:Musa;
    rdfs:range xsd:string;
    cco:section "6.6.10"
    .

cco:antherExsertionMusa a rdf:Property;
    rdfs:label "Anther exsertion"@en;
    rdfs:comment """
In relation to the base of the lobes on the compound tepal
1 Exserted
2 Same level
3 Inserted
    """@en;
    rdfs:domain cco:Musa;
    rdfs:range xsd:string;
    cco:section "6.6.11"
    .

cco:filamentColourMusa a rdf:Property;
    rdfs:label "Filament colour"@en;
    rdfs:comment """
1 White
2 Cream
3 Yellow
    """@en;
    rdfs:domain cco:Musa;
    rdfs:range xsd:string;
    cco:section "6.6.12"
    .

cco:antherColourMusa a rdf:Property;
    rdfs:label "Anther colour"@en;
    rdfs:comment """
Observed on the face opposite to the dehiscence split of the anther (dorsal face).
1 White 
2 Cream 
3 Yellow 
4 Grey 
5 Brown/rusty brown
6 Pink/pink-purple
7 Black (anthers aborted)
8 Other
    """@en;
    rdfs:domain cco:Musa;
    rdfs:range xsd:string;
    cco:section "6.6.13"
    .

cco:pollenSacColourMusa a rdf:Property;
    rdfs:label "Pollen sac colour"@en;
    rdfs:comment """
Recorded at the line where the anther splits to release pollen. 
1 White 
2 Cream 
3 Yellow 
4 Brown/rusty brown
5 Pink/pink-purple
6 Red-purple
7 Other
    """@en;
    rdfs:domain cco:Musa;
    rdfs:range xsd:string;
    cco:section "6.6.14"
    .

cco:pollenVitalityMusa a rdf:Property;
    rdfs:label "Pollen vitality"@en;
    rdfs:comment """
Percentage of deformed and/or aborted grains in relation to normal grains. Use
Alexander’s pollen viability assessment method
    """@en;
    rdfs:domain cco:Musa;
    rdfs:range xsd:string;
    cco:section "6.6.15"
    .

cco:styleBasicColourMusa a rdf:Property;
    rdfs:label "Style basic colour"@en;
    rdfs:comment """
Do not refer to the minute blotches which can be present on the style
1 White 
2 Cream 
3 Red-purple
4 Other
    """@en;
    rdfs:domain cco:Musa;
    rdfs:range xsd:string;
    cco:section "6.6.16"
    .

cco:pigmentationOnStyleMusa a rdf:Property;
    rdfs:label "Pigmentation on style"@en;
    rdfs:comment """
1 Without pigmentation
2 Purple
    """@en;
    rdfs:domain cco:Musa;
    rdfs:range xsd:string;
    cco:section "6.6.17"
    .

cco:styleExsertionMusa a rdf:Property;
    rdfs:label "Style exsertion"@en;
    rdfs:comment """
In relation to the base of the lobes on the compound tepal
1 Exserted
2 Same level
3 Inserted
    """@en;
    rdfs:domain cco:Musa;
    rdfs:range xsd:string;
    cco:section "6.6.18"
    .

cco:styleShapeMusa a rdf:Property;
    rdfs:label "Style shape"@en;
    rdfs:comment """
1 Straight 
2 Curved under stigma 
3 Curved at the base
4 Curved twice
5 Other
    """@en;
    rdfs:domain cco:Musa;
    rdfs:range xsd:string;
    foaf:depiction <http://www.agrobiodiversity.org/files/styleShapeMusa.png>;
    cco:section "6.6.19"
    .
cco:stigmaColourMusa a rdf:Property;
    rdfs:label "Stigma colour"@en;
    rdfs:comment """
1 Cream
2 Yellow
3 Pink/pink-purple
4 Bright yellow
5 Orange
6 Other
    """@en;
    rdfs:domain cco:Musa;
    rdfs:range xsd:string;
    cco:section "6.6.20"
    .

cco:ovaryShapeMusa a rdf:Property;
    rdfs:label "Ovary shape"@en;
    rdfs:comment """
1 Straight
2 Arched
    """@en;
    rdfs:domain cco:Musa;
    rdfs:range xsd:string;
    foaf:depiction <http://www.agrobiodiversity.org/files/ovaryShapeMusa.png>;
    cco:section "6.6.21"
    .

cco:ovaryBasicColourMusa a rdf:Property;
    rdfs:label "Ovary basic colour"@en;
    rdfs:comment """
1 White 
2 Cream 
3 Yellow 
4 Green
5 Other
    """@en;
    rdfs:domain cco:Musa;
    rdfs:range xsd:string;
    cco:section "6.6.22"
    .

cco:ovaryPigmentationMusa a rdf:Property;
    rdfs:label "Ovary pigmentation"@en;
    rdfs:comment """
1 Very few or no visible sign of pigmentation
2 With red-purple
    """@en;
    rdfs:domain cco:Musa;
    rdfs:range xsd:string;
    cco:section "6.6.23"
    .

cco:dominantColourOfMaleFlowerMusa a rdf:Property;
    rdfs:label "Dominant colour of male flower"@en;
    rdfs:comment """
1 White 
2 Cream 
3 Yellow 
4 Pink/pink-purple
5 Red-purple
6 Other
    """@en;
    rdfs:domain cco:Musa;
    rdfs:range xsd:string;
    cco:section "6.6.24"
    .

 
cco:irregularFlowersMusa a rdf:Property;
    rdfs:label "Irregular flowers"@en;
    rdfs:comment """
Record number of flowers per cluster with an abnormal number of stamens, fusion
of free and compound tepal, etc.
    """@en;
    rdfs:domain cco:Musa;
    rdfs:range xsd:string;
    cco:section "6.6.25"
    .

cco:arrangementOfOvulesMusa a rdf:Property;
    rdfs:label "Arrangement of ovules"@en;
    rdfs:comment """
Observed soon after flowering and before the fruit fills. Observe a cross-section of
a fruit.
1 Two rowed
2 Four-rowed (more or less)
    """@en;
    rdfs:domain cco:Musa;
    rdfs:range xsd:string;
    foaf:depiction <http://www.agrobiodiversity.org/files/arrangementOfOvulesMusa.png>;
    cco:section "6.6.26"
    .

cco:fruitPositionMusa a rdf:Property;
    rdfs:label "Fruit position"@en;
    rdfs:comment """
Recorded only on fruits arranged symmetrically around the stalk
1 Curved towards stalk
2 Parallel to the stalk
3 Curved upward (obliquely, at a 45°angle upward)
4 Perpendicular to the stalk
5 Pendant
    """@en;
    rdfs:domain cco:Musa;
    rdfs:range xsd:string;
    cco:section "6.7.1"
    .

cco:numberOfFruitsMusa a rdf:Property;
    rdfs:label "Number of fruits"@en;
    rdfs:comment """
Observed on the mid-hand of the bunch
1 ≤12
2 13-16
3 ≥17
    """@en;
    rdfs:domain cco:Musa;
    rdfs:range xsd:string;
    cco:section "6.7.2"
    .

cco:fruitLengthMusa a rdf:Property;
    rdfs:label "Fruit length"@en;
    rdfs:comment """
Measured as the internal arc of the fruit, without pedicel
1 ≤15 cm
2 16- 20 cm
3 21- 25 cm
4 26- 30 cm
5 ≥31 cm
    """@en;
    rdfs:domain cco:Musa;
    rdfs:range xsd:string;
    cco:section "6.7.3"
    .

cco:fruitShapeLongitudinalCurvatureMusa a rdf:Property;
    rdfs:label "Fruit shape longitudinal curvature"@en;
    rdfs:comment """
1 Straight (or slightly curved)
2 Straight in the distal part
3 Curved (sharp curve)
4 Curved in ‘S’ shape (double curvature)
5 Other (specify in descriptor Notes, 6.8)
    """@en;
    rdfs:domain cco:Musa;
    rdfs:range xsd:string;
    foaf:depiction <http://www.agrobiodiversity.org/files/fruitShapeLongitudinalCurvatureMusa.png>;
    cco:section "6.7.4"
    .

cco:transverseSectionOfFruitMusa a rdf:Property;
    rdfs:label "Transverse section of fruit"@en;
    rdfs:comment """
Observed on mature fruit (‘ready to eat’ - ripe but not over-ripe, full yellow stage).
1 Pronounced ridges
2 Slightly ridged
3 Rounded
    """@en;
    rdfs:domain cco:Musa;
    rdfs:range xsd:string;
    foaf:depiction <http://www.agrobiodiversity.org/files/transverseSectionOfFruitMusa.png>;
    cco:section "6.7.5"
    .
cco:fruitApexMusa a rdf:Property;
    rdfs:label "Fruit apex"@en;
    rdfs:comment """
Observed at the distal end of the fruit. 
1 Pointed
2 Lengthily pointed
3 Blunt-tipped
4 Bottle-necked
5 Rounded
    """@en;
    rdfs:domain cco:Musa;
    rdfs:range xsd:string;
    foaf:depiction <http://www.agrobiodiversity.org/files/fruitApexMusa.png>;
    cco:section "6.7.6"
    .

cco:remainsOfFlowerRelictsAtFruitApexMusa a rdf:Property;
    rdfs:label "Remains of flower relicts at fruit apex"@en;
    rdfs:comment """
Observed at the distal end of the fruit. 
1 Without any floral relicts
2 Persistent style
3 Base of the style prominent
    """@en;
    rdfs:domain cco:Musa;
    rdfs:range xsd:string;
    foaf:depiction <http://www.agrobiodiversity.org/files/remainsOfFlowerRelictsAtFruitApexMusa.png>;
    cco:section "6.7.7"
    .

cco:fruitPedicelLengthMusa a rdf:Property;
    rdfs:label "Fruit pedicel length"@en;
    rdfs:comment """
1 ≤10 mm
2 11 to 20 mm
3 ≥21 mm
    """@en;
    rdfs:domain cco:Musa;
    rdfs:range xsd:string;
    cco:section "6.7.8"
    .

cco:fruitPedicelWidthMusa a rdf:Property;
    rdfs:label "Fruit pedicel width"@en;
    rdfs:comment """
1 <5 mm
2 5 to 10 mm
3 >10 mm
    """@en;
    rdfs:domain cco:Musa;
    rdfs:range xsd:string;
    cco:section "6.7.9"
    .

cco:pedicelSurfaceMusa a rdf:Property;
    rdfs:label "Pedicel surface"@en;
    rdfs:comment """
1 Hairless
2 Hairy
    """@en;
    rdfs:domain cco:Musa;
    rdfs:range xsd:string;
    cco:section "6.7.10"
    .

cco:fusionOfPedicelsMusa a rdf:Property;
    rdfs:label "Fusion of pedicels"@en;
    rdfs:comment """
(Before joining the crown)
1 Very partially or no visible sign of fusion
2 Partially fused
3 Totally fused
    """@en;
    rdfs:domain cco:Musa;
    rdfs:range xsd:string;
    cco:section "6.7.11"
    .

cco:immatureFruitPeelColourMusa a rdf:Property;
    rdfs:label "Immature fruit peel colour"@en;
    rdfs:comment """
Recorded on the youngest hand of the bunch, before maturity. 
1 Yellow
2 Light green
3 Green
4 Green and pink, red or purple
5 Silvery
6 Dark green
7 Brown/rusty brown
8 Pink, red or purple
9 Black
10 Other
    """@en;
    rdfs:domain cco:Musa;
    rdfs:range xsd:string;
    cco:section "6.7.12"
    .

cco:matureFruitPeelColourMusa a rdf:Property;
    rdfs:label "Mature fruit peel colour"@en;
    rdfs:comment """
Recorded at fruit maturity (ripe, but not over-ripe; full yellow stage). 
1 Yellow
2 Bright yellow
3 Orange
4 Grey spots
5 Brown/rusty-brown
6 Orange red, red or pink/pink purple
7 Red-purple
8 Black
9 Other
    """@en;
    rdfs:domain cco:Musa;
    rdfs:range xsd:string;
    cco:section "6.7.13"
    .

cco:fruitPeelThicknessMusa a rdf:Property;
    rdfs:label "Fruit peel thickness"@en;
    rdfs:comment """
Recorded at fruit maturity (‘ready to eat’ ripe, but not over-ripe; full yellow stage)
1 Two or less
2 Three or more
    """@en;
    rdfs:domain cco:Musa;
    rdfs:range xsd:string;
    cco:section "6.7.14"
    .

cco:adherenceOfTheFruitPeelMusa a rdf:Property;
    rdfs:label "Adherence of the fruit peel"@en;
    rdfs:comment """
Recorded at fruit maturity (ripe, but not over-ripe; full yellow stage)
1 Fruit peels easily
2 Fruit does not peel easily
    """@en;
    rdfs:domain cco:Musa;
    rdfs:range xsd:string;
    cco:section "6.7.15"
    .

cco:cracksInFruitPeelMusa a rdf:Property;
    rdfs:label "Cracks in fruit peel"@en;
    rdfs:comment """
Recorded at fruit maturity if the peel splits without mechanical damage
1 Without cracks
2 Cracked
    """@en;
    rdfs:domain cco:Musa;
    rdfs:range xsd:string;
    cco:section "6.7.16"
    .

cco:pulpInFruitMusa a rdf:Property;
    rdfs:label "Pulp in fruit"@en;
    rdfs:comment """
1 Without pulp
2 With pulp
    """@en;
    rdfs:domain cco:Musa;
    rdfs:range xsd:string;
    cco:section "6.7.17"
    .

cco:pulpColourBeforeMaturityMusa a rdf:Property;
    rdfs:label "Pulp colour before maturity"@en;
    rdfs:comment """
Recorded on youngest hand of the bunch. 
1 White
2 Cream
3 Ivory
4 Yellow
5 Orange
6 Beige-pink
7 Other
    """@en;
    rdfs:domain cco:Musa;
    rdfs:range xsd:string;
    cco:section "6.7.18"
    .

cco:pulpColourAtMaturityMusa a rdf:Property;
    rdfs:label "Pulp colour at maturity"@en;
    rdfs:comment """
(Ripe, but not over-ripe; full yellow stage)
1 White
2 Cream
3 Ivory
4 Yellow
5 Orange
6 Beige-pink
7 Other
    """@en;
    rdfs:domain cco:Musa;
    rdfs:range xsd:string;
    cco:section "6.7.19"
    .

cco:fruitsFallFromHandsMusa a rdf:Property;
    rdfs:label "Fruits fall from hands"@en;
    rdfs:comment """
Observed at fruit maturity
1 Persistent
2 Deciduous
    """@en;
    rdfs:domain cco:Musa;
    rdfs:range xsd:string;
    cco:section "6.7.20"
    .
cco:fleshTextureMusa a rdf:Property;
    rdfs:label "Flesh texture"@en;
    rdfs:comment """
1 Firm
2 Soft
    """@en;
    rdfs:domain cco:Musa;
    rdfs:range xsd:string;
    cco:section "6.7.21"
    .

cco:predominantTasteMusa a rdf:Property;
    rdfs:label "Predominant taste"@en;
    rdfs:comment """
1 Astringent (like cooking banana)
2 Mild, slightly tasty or tasteless
3 Sweet (like Cavendish)
4 Sugary (like ‘Pisang Mas’)
5 Sweet and acidic (apple like)
6 Other
    """@en;
    rdfs:domain cco:Musa;
    rdfs:range xsd:string;
    cco:section "6.7.22"
    .

cco:presenceOfSeedWithSourceOfPollenMusa a rdf:Property;
    rdfs:label "Presence of seed with source of pollen"@en;
    rdfs:comment """
Record the number of seeds only if there exists in the vicinity of the plant a
population of wild relatives, or male fertile hybrids (pollen sources), or if the female
flowers are artificially pollinated
1 <5
2 5-20
3 >20
    """@en;
    rdfs:domain cco:Musa;
    rdfs:range xsd:string;
    cco:section "6.7.23"
    .

cco:seedSurfaceMusa a rdf:Property;
    rdfs:label "Seed surface"@en;
    rdfs:comment """
1 Smooth
2 Wrinkled
    """@en;
    rdfs:domain cco:Musa;
    rdfs:range xsd:string;
    cco:section "6.7.24"
    .

cco:seedShapeMusa a rdf:Property;
    rdfs:label "Seed shape"@en;
    rdfs:comment """
1 Flat
2 Angular (more or less pyramidal)
3 Globular (spherical)
4 Rounded (but not completely spherical)
    """@en;
    rdfs:domain cco:Musa;
    rdfs:range xsd:string;
    cco:section "6.7.25"
    .

